dataplane/Timely_Stream.thy
@@ -8,10 +8,10 @@ begin
 
 datatype ('t :: order, 'd) event = Data (time: 't) (data: 'd) | Drop (time: 't) | Mint (time: 't)
 
-coinductive monotone :: "('t::order, 'd) event llist \<Rightarrow> 't multiset \<Rightarrow> bool" where
-  LNil: "monotone LNil {#}"
-| LConsDrop: "\<lbrakk> t \<in># C ; monotone xs (C - {# t #})\<rbrakk> \<Longrightarrow> monotone (LCons (Drop t) xs) C"
-| LConsMint: "\<lbrakk> t' \<in># C ; t' \<le> t ; monotone xs (C + {# t #}  )\<rbrakk> \<Longrightarrow> monotone (LCons (Mint t) xs) C"
-| LConsData: "\<lbrakk> t \<in># C  ; monotone xs C \<rbrakk> \<Longrightarrow> monotone (LCons (Data t d) xs) C" 
+coinductive timely_monotone :: "('t::order, 'd) event llist \<Rightarrow> 't multiset \<Rightarrow> bool" where
+  LNil: "timely_monotone LNil {#}"
+| LConsDrop: "\<lbrakk> t \<in># C ; timely_monotone xs (C - {# t #})\<rbrakk> \<Longrightarrow> timely_monotone (LCons (Drop t) xs) C"
+| LConsMint: "\<lbrakk> t' \<in># C ; t' \<le> t ; timely_monotone xs (C + {# t #}  )\<rbrakk> \<Longrightarrow> timely_monotone (LCons (Mint t) xs) C"
+| LConsData: "\<lbrakk> t \<in># C  ; timely_monotone xs C \<rbrakk> \<Longrightarrow> timely_monotone (LCons (Data t d) xs) C" 
 
 end
